src/Analysis/Domains/Ivl_Exec.thy
@@ -1,0 +1,201 @@
+theory Ivl_Exec
+  imports Exec_Bridge Interval_Domain
+begin
+
+section \<open>Interval executable transfer mirror\<close>
+
+instance ivl :: bounded_warrowing ..
+
+
+text \<open>
+  Executable mirror of @{const ivl_tf} on @{typ "ivl st"}, following
+  the sign-domain pattern in @{file "Sign_Exec.thy"}.  Commutation lemmas hook
+  into the generic @{theory Voblint_Analysis.Exec_Bridge} transport; no certified
+  end-to-end soundness theory yet (cf.\ @{file "Sign_Exec_Sound.thy"}).
+\<close>
+
+lemma fun_of_st_update:
+  "fun_of_st (update_st s x v) = (fun_of_st s)(x := v)"
+  by (rule ext) (metis fun_upd_apply lookup_update_diff lookup_update_same)
+
+subsection \<open>Backward filter mirror on @{typ "ivl st"}\<close>
+
+fun afilter_ivl_st :: "aexp \<Rightarrow> ivl \<Rightarrow> ivl st \<Rightarrow> ivl st" where
+    "afilter_ivl_st (BaseN (AExp.V x)) a s =
+       update_st s x (meet_ivl a (lookup_st s x))"
+  | "afilter_ivl_st (Plus e1 e2) a s =
+       (let (a1, a2) = inv_plus_ivl a (aval_ivl e1 (lookup_st s)) (aval_ivl e2 (lookup_st s))
+        in afilter_ivl_st e1 a1 (afilter_ivl_st e2 a2 s))"
+  | "afilter_ivl_st (Minus e1 e2) a s =
+       (let (a1, a2) = inv_minus_ivl a (aval_ivl e1 (lookup_st s)) (aval_ivl e2 (lookup_st s))
+        in afilter_ivl_st e1 a1 (afilter_ivl_st e2 a2 s))"
+  | "afilter_ivl_st (Times e1 e2) a s =
+       (let (a1, a2) = inv_times_ivl a (aval_ivl e1 (lookup_st s)) (aval_ivl e2 (lookup_st s))
+        in afilter_ivl_st e1 a1 (afilter_ivl_st e2 a2 s))"
+  | "afilter_ivl_st _ a s = s"
+
+fun bfilter_ivl_st :: "bexp \<Rightarrow> bool \<Rightarrow> ivl st \<Rightarrow> ivl st" where
+    "bfilter_ivl_st (Less e1 e2) res s =
+       (let (a1, a2) = inv_less_ivl res (aval_ivl e1 (lookup_st s)) (aval_ivl e2 (lookup_st s))
+        in afilter_ivl_st e1 a1 (afilter_ivl_st e2 a2 s))"
+  | "bfilter_ivl_st (Not b) res s = bfilter_ivl_st b (\<not> res) s"
+  | "bfilter_ivl_st (And b1 b2) True s =
+       bfilter_ivl_st b1 True (bfilter_ivl_st b2 True s)"
+  | "bfilter_ivl_st (And b1 b2) False s =
+       bfilter_ivl_st b1 False s \<squnion> bfilter_ivl_st b2 False s"
+  | "bfilter_ivl_st (Or b1 b2) True s =
+       bfilter_ivl_st b1 True s \<squnion> bfilter_ivl_st b2 True s"
+  | "bfilter_ivl_st (Or b1 b2) False s =
+       bfilter_ivl_st b1 False (bfilter_ivl_st b2 False s)"
+  | "bfilter_ivl_st (Eq e1 e2) True s =
+       (let a = meet_ivl (aval_ivl e1 (lookup_st s)) (aval_ivl e2 (lookup_st s))
+        in afilter_ivl_st e1 a (afilter_ivl_st e2 a s))"
+  | "bfilter_ivl_st _ _ s = s"
+
+lemma afilter_ivl_st_commute:
+  "fun_of_st (afilter_ivl_st e a s) = afilter_ivl e a (fun_of_st s)"
+proof (induction e arbitrary: a s)
+  case (BaseN x)
+  show ?case by (cases x; simp add: fun_of_st_update)
+next
+  case (Plus e1 e2)
+  show ?case by (simp add: Plus.IH)
+next
+  case (Minus e1 e2)
+  show ?case by (simp add: Minus.IH)
+next
+  case (Times e1 e2)
+  show ?case by (simp add: Times.IH)
+qed
+
+lemma bfilter_ivl_st_commute:
+  "fun_of_st (bfilter_ivl_st b res s) = bfilter_ivl b res (fun_of_st s)"
+proof (induction b arbitrary: res s)
+  case (BaseB x)
+  then show ?case by simp
+next
+  case (Not b)
+  then show ?case by simp
+next
+  case (And b1 b2)
+  show ?case
+  proof (cases res)
+    case True
+    then show ?thesis by (simp add: And.IH)
+  next
+    case False
+    then show ?thesis by (simp add: And.IH)
+  qed
+next
+  case (Or b1 b2)
+  show ?case
+  proof (cases res)
+    case True
+    then show ?thesis by (simp add: Or.IH)
+  next
+    case False
+    then show ?thesis by (simp add: Or.IH)
+  qed
+next
+  case (Less e1 e2)
+  then show ?case by (simp add: afilter_ivl_st_commute split: prod.splits)
+next
+  case (Eq e1 e2)
+  show ?case
+  proof (cases res)
+    case True
+    then show ?thesis by (simp add: afilter_ivl_st_commute Let_def)
+  next
+    case False
+    then show ?thesis by simp
+  qed
+qed
+
+definition assume_ivl_st :: "bexp \<Rightarrow> ivl st \<Rightarrow> ivl st" where
+  "assume_ivl_st b s = bfilter_ivl_st b True s"
+
+definition assume_not_ivl_st :: "bexp \<Rightarrow> ivl st \<Rightarrow> ivl st" where
+  "assume_not_ivl_st b s = bfilter_ivl_st b False s"
+
+lemma assume_ivl_st_commute:
+  "fun_of_st (assume_ivl_st b s) = assume_ivl b (fun_of_st s)"
+  by (simp add: assume_ivl_st_def assume_ivl_def bfilter_ivl_st_commute)
+
+lemma assume_not_ivl_st_commute:
+  "fun_of_st (assume_not_ivl_st b s) = assume_not_ivl b (fun_of_st s)"
+  by (simp add: assume_not_ivl_st_def assume_not_ivl_def bfilter_ivl_st_commute)
+
+subsection \<open>Enter mirror\<close>
+
+lemma fun_rep_enter_ivl_rep:
+  "fun_rep_st ((\<lambda>(dl, dg, ps). (Ivl MinInf PlusInf, dg, filter (\<lambda>(x, _). is_global x) ps)) r)
+   = (\<lambda>x. if is_global x then fun_rep_st r x else Ivl MinInf PlusInf)"
+proof -
+  obtain dl dg ps where r: "r = (dl, dg, ps)" using prod_cases3 by blast
+  show ?thesis unfolding r
+    by (rule ext) (auto simp: map_of_filter_key split: option.split)
+qed
+
+lift_definition enter_ivl_st :: "ivl st \<Rightarrow> ivl st"
+  is "\<lambda>(dl, dg, ps). (Ivl MinInf PlusInf, dg, filter (\<lambda>(x, _). is_global x) ps)"
+  by (auto simp: eq_st_def fun_rep_enter_ivl_rep fun_eq_iff)
+
+lemma enter_ivl_st_commute:
+  "fun_of_st (enter_ivl_st s) = enter_ivl (fun_of_st s)"
+  unfolding enter_ivl_def
+  by transfer (simp add: fun_rep_enter_ivl_rep)
+
+subsection \<open>Executable transfer function and seeds\<close>
+
+fun ivl_tf_st :: "edge_action \<Rightarrow> ivl st \<Rightarrow> ivl st" where
+    "ivl_tf_st EA_Nop s = s"
+  | "ivl_tf_st (EA_Assign x a) s = update_st s x (aval_ivl a (lookup_st s))"
+  | "ivl_tf_st (EA_Assume b) s = assume_ivl_st b s"
+  | "ivl_tf_st (EA_AssumeNot b) s = assume_not_ivl_st b s"
+  | "ivl_tf_st EA_Enter s = enter_ivl_st s"
+
+lift_definition top_ivl_st :: "ivl st" is "(Ivl MinInf PlusInf, Ivl MinInf PlusInf, [])" .
+
+lift_definition cinit_ivl_st :: "ivl st" is "(Ivl MinInf PlusInf, Ivl (Fin 0) (Fin 0), [])" .
+
+lemma lookup_cinit_ivl_st [simp]:
+  "lookup_st cinit_ivl_st x = (if is_global x then Ivl (Fin 0) (Fin 0) else Ivl MinInf PlusInf)"
+  by transfer (auto split: if_splits)
+
+lemma fun_of_st_cinit_ivl_st:
+  "fun_of_st cinit_ivl_st = (\<lambda>x. if is_global x then Ivl (Fin 0) (Fin 0) else Ivl MinInf PlusInf)"
+  by (rule ext) simp
+
+lemma lookup_top_ivl_st [simp]: "lookup_st top_ivl_st x = Ivl MinInf PlusInf"
+  by transfer simp
+
+lemma fun_of_st_top_ivl_st:
+  "fun_of_st top_ivl_st = (\<lambda>_. Ivl MinInf PlusInf)"
+  by (rule ext) simp
+
+theorem ivl_tf_st_commute:
+  "fun_of_st (ivl_tf_st a s) = apply_tf ivl_tf a (fun_of_st s)"
+proof (cases a)
+  case EA_Nop
+  then show ?thesis by simp
+next
+  case (EA_Assign x e)
+  then show ?thesis
+    by (simp add: ivl_tf_def assign_ivl_def fun_of_st_update)
+next
+  case (EA_Assume b)
+  then show ?thesis
+    by (simp add: ivl_tf_def assume_ivl_st_commute)
+next
+  case (EA_AssumeNot b)
+  then show ?thesis
+    by (simp add: ivl_tf_def assume_not_ivl_st_commute)
+next
+  case EA_Enter
+  then show ?thesis by (simp add: ivl_tf_def enter_ivl_st_commute)
+qed
+
+value "lookup_st (ivl_tf_st (EA_Assume (Less (IMP2_Syntax.V ''x'') (IMP2_Syntax.N 20)))
+           (update_st top_ivl_st ''x'' (Ivl (Fin 0) (Fin 20)))) ''x''"
+
+end
